theories/input_lang/interp.v
@@ -33,8 +33,8 @@ Section constructors.
   Definition INPUT : (natO -n> IT) -n> IT.
   Proof using E subEff0.
     simple refine (λne k, Vis (E:=E) (subEff_opid (()))
-                            (subEff_conv_ins (F:=inputE) (op:=(())) ())
-                            (NextO ◎ k ◎ subEff_conv_outs2 (F:=inputE) (op:=(())))).
+                            (subEff_ins (F:=inputE) (op:=(())) ())
+                            (NextO ◎ k ◎ (subEff_outs (F:=inputE) (op:=(())))^-1)).
     solve_proper.
   Defined.
 
@@ -543,15 +543,15 @@ Section interp.
     (σ σ' : stateO) (σr : gState_rest sR_idx rs ♯ IT) n :
     head_step e σ e' σ' (n,1) →
     reify (gReifiers_sReifier rs)
-      (interp_expr (fill K e) env)  (gState_recomp σr (subR_conv_state σ))
-      ≡ (gState_recomp σr (subR_conv_state σ'), Tick_n n $ interp_expr (fill K e') env).
+      (interp_expr (fill K e) env)  (gState_recomp σr (sR_state σ))
+      ≡ (gState_recomp σr (sR_state σ'), Tick_n n $ interp_expr (fill K e') env).
   Proof.
     inversion 1; simplify_eq.
     trans (reify (gReifiers_sReifier rs) (interp_ectx K env (interp_expr Input env))
-             (gState_recomp σr (subR_conv_state σ))).
+             (gState_recomp σr (sR_state σ))).
     { f_equiv. by rewrite interp_ectx_fill. }
     simpl.
-    trans (reify (gReifiers_sReifier rs) (INPUT (interp_ectx K env ◎ Nat)) (gState_recomp σr (subR_conv_state σ))).
+    trans (reify (gReifiers_sReifier rs) (INPUT (interp_ectx K env ◎ Nat)) (gState_recomp σr (sR_state σ))).
     { f_equiv; eauto.
       by rewrite interp_ectx_INPUT. }
     rewrite reify_vis_eq //; last first.
@@ -566,8 +566,8 @@ Section interp.
   Lemma soundness {S} (e1 e2 : expr S) σ1 σ2 (σr : gState_rest sR_idx rs ♯ IT) n m env :
     prim_step e1 σ1 e2 σ2 (n,m) →
     ssteps (gReifiers_sReifier rs)
-              (interp_expr e1 env) (gState_recomp σr (subR_conv_state σ1))
-              (interp_expr e2 env) (gState_recomp σr (subR_conv_state σ2)) n.
+              (interp_expr e1 env) (gState_recomp σr (sR_state σ1))
+              (interp_expr e2 env) (gState_recomp σr (sR_state σ2)) n.
   Proof.
     Opaque gState_decomp gState_recomp.
     inversion 1; simplify_eq/=.
